coq/set/Core/Compatible.v
@@ -1,5 +1,49 @@
+Require Import Peano_dec.
+
 Require Import Core.Set.
+Require Import Core.Elem.
 Require Import Core.Equal.
+Require Import Core.Syntax.
+Require Import Core.Semantics.
+Require Import Core.Environment.
 
 Definition compatible (P:set -> Prop) : Prop :=
     forall (x y:set), x == y -> P x -> P y.
+
+(* Any predicate obtained by a formula is a compatible predicate.               *)
+Theorem formulaCompatible : forall (e:Env) (n:nat) (p:Formula),
+    compatible (eval' e n p). 
+Proof.
+    intros e n p. revert e n. induction p as [|k m|p1 IH1 p2 IH2|m p1 IH1];
+    intros e n; unfold compatible, eval'; intros x y E; simpl; intros H.
+    - assumption.
+    - apply equal_l with (bind e n x k). 
+        + apply bindEqual. assumption.
+        + apply equal_r with (bind e n x m).
+            { apply bindEqual. assumption. }
+            { assumption. }
+    - unfold compatible, eval' in IH1. unfold compatible, eval' in IH2. intros H'.
+      apply IH2 with x.
+        + assumption.
+        + apply H. apply IH1 with y.
+            { apply equalSym. assumption. }
+            { assumption. }
+    - intros z. unfold compatible, eval' in IH1. 
+      destruct (eq_nat_dec m n) as [H'|H'].
+        + subst. apply (evalEnvEqual (bind (bind e n y) n z) (bind e n z)).
+            { apply bindOver. }
+            { apply (evalEnvEqual (bind (bind e n x) n z) (bind e n z)).
+                { apply bindOver. }
+                { apply H. }}
+        + apply (evalEnvEqual 
+            (bind (bind e n y) m z)
+            (bind (bind e m z) n y)).
+            { apply bindPermute. assumption. }
+            { apply IH1 with x.
+                { assumption. }
+                { apply (evalEnvEqual 
+                    (bind (bind e n x) m z)
+                    (bind (bind e m z) n x)).
+                    { apply bindPermute. assumption. }
+                    { apply H. }}}
+Qed.
